Quick_Sort.thy
@@ -3,22 +3,44 @@ imports Sorting
 begin
 
 lemma multiset_partition:
-  "multiset_of (fst (partition f xs)) + multiset_of (snd (partition f xs)) = multiset_of xs"
+  "mset (fst (partition f xs)) + mset (snd (partition f xs)) = mset xs"
 by (induction xs) (auto simp: algebra_simps)
 
 fun quicksort :: "'a::linorder list \<Rightarrow> 'a list" where
 "quicksort [] = []" |
 "quicksort (x # xs) = (let (as, bs) = partition (\<lambda>y. y \<le> x) xs in quicksort as @ x # quicksort bs)"
 
-interpretation quick_sort!: sorting quicksort
+declare sorted.empty[simp]
+declare sorted.single[simp]
+
+lemma sorted_cons_iff: "sorted (x # xs) \<longleftrightarrow> (\<forall>x' \<in> set xs. x \<le> x') \<and> sorted xs"
+sorry
+
+lemma sorted_appI: "sorted xs \<Longrightarrow> sorted ys \<Longrightarrow> \<forall>x \<in> set xs. \<forall>y \<in> set ys. x \<le> y \<Longrightarrow> sorted (xs @ ys)"
+  sorry
+
+global_interpretation quick_sort: sorting quicksort
 proof
   fix xs :: "'a::linorder list"
-  show "multiset_of (quicksort xs) = multiset_of xs"
+  show "mset (quicksort xs) = mset xs"
     by (induction xs rule: quicksort.induct)
        (auto simp: multiset_partition[simplified] algebra_simps)
 
   show "sorted (quicksort xs)"
-    sorry
+    apply (induction xs rule: quicksort.induct)
+     apply simp
+    unfolding quicksort.simps
+    apply (case_tac "partition (\<lambda>y. y \<le> x) xs")
+    apply (simp only: Let_def)
+    unfolding prod.case
+    apply (rule sorted_appI)
+      apply simp
+     apply (subst sorted_cons_iff)
+     apply (rule conjI)
+    subgoal sorry
+     apply simp
+    subgoal sorry
+    done
 qed
 
 end
